p256: move Spec.ECDSA and and Spec.DH to Spec.P256

specs/ecdsap256/Spec.P256.fst
@@ -5,173 +5,16 @@ open FStar.Mul
 open Lib.IntTypes
 open Lib.Sequence
 
+open Spec.Hash.Definitions
+
 module M = Lib.NatMod
+module BSeq = Lib.ByteSequence
+
+include Spec.P256.PointOps
 
 #set-options "--z3rlimit 50 --fuel 0 --ifuel 0"
 
-(* https://eprint.iacr.org/2013/816.pdf *)
-
-///  Base field
-
-// 0xffffffff00000001000000000000000000000000ffffffffffffffffffffffff
-let prime: (a:pos{8 < a && a < pow2 256}) =
-  assert_norm (pow2 256 - pow2 224 + pow2 192 + pow2 96 - 1 > 8);
-  assert_norm (pow2 256 - pow2 224 + pow2 192 + pow2 96 - 1 < pow2 256);
-  pow2 256 - pow2 224 + pow2 192 + pow2 96 - 1
-
-let felem = x:nat{x < prime}
-let zero : felem = 0
-let one  : felem = 1
-
-let fadd (x y:felem) : felem = (x + y) % prime
-let fsub (x y:felem) : felem = (x - y) % prime
-let fmul (x y:felem) : felem = (x * y) % prime
-let finv (a:felem) : felem = M.pow_mod #prime a (prime - 2)
-let fsqrt (a:felem) : felem = M.pow_mod #prime a ((prime + 1) / 4)
-
-let ( +% ) = fadd
-let ( -% ) = fsub
-let ( *% ) = fmul
-
-//---------------------------------------
-// TODO: remove
-val pow: a:nat -> b:nat -> nat
-let rec pow a b =
-  if b = 0 then 1
-  else a * (pow a (b - 1))
-
-type elem (n:pos) = x:nat{x < n}
-let mul_n (#n:pos) (x:elem n) (y:elem n) : elem n = (x * y) % n
-
-val exp: #n: pos -> a: elem n -> b: pos -> Tot (elem n) (decreases b)
-let rec exp #n a b =
-  if b = 1 then a
-  else
-    if b % 2 = 0 then exp (mul_n a a) (b / 2)
-    else mul_n a (exp (mul_n a a) (b / 2))
-
-let modp_inv_prime (prime: pos {prime > 3}) (x: elem prime) : Tot (elem prime) =
-  (exp #prime x (prime - 2)) % prime
-
-let modp_inv2_prime (x: int) (p: nat {p > 3}) : Tot (elem p) = modp_inv_prime p (x % p)
-
-let modp_inv2 (x: nat) : Tot (elem prime) =
-  assert_norm(prime > 3);
-  modp_inv2_prime x prime
-//---------------------------------------
-
-
-///  Scalar field
-
-// Group order
-// 0xffffffff00000000ffffffffffffffffbce6faada7179e84f3b9cac2fc632551
-let order: (a:pos{a < pow2 256}) =
-  assert_norm (115792089210356248762697446949407573529996955224135760342422259061068512044369 < pow2 256);
-  115792089210356248762697446949407573529996955224135760342422259061068512044369
-
-let qelem = x:nat{x < order}
-let qadd (x y:qelem) : qelem = (x + y) % order
-let qmul (x y:qelem) : qelem = (x * y) % order
-let qinv (x:qelem) : qelem = M.pow_mod #order x (order - 2)
-
-let ( +^ ) = qadd
-let ( *^ ) = qmul
-
-
-///  Elliptic curve `y^2 = x^3 + a * x + b`
-
-let point_nat = tuple3 nat nat nat
-let jacob_point = p:point_nat{let (a, b, c) = p in
-  a < prime /\ b < prime /\ c < prime}
-
-// let aff_point = felem & felem           // Affine point
-// let jacob_point = felem & felem & felem // Jacobian coordinates
-
-let a_coeff : felem = (-3) % prime
-let b_coeff : felem =
-  assert_norm (41058363725152142129326129780047268409114441015993725554835256314039467401291 < prime);
-  41058363725152142129326129780047268409114441015993725554835256314039467401291
-
-// Base point
-let g_x : felem =
-  let x = 0x6B17D1F2E12C4247F8BCE6E563A440F277037D812DEB33A0F4A13945D898C296 in
-  assert_norm (x < prime); x
-let g_y : felem =
-  let y = 0x4FE342E2FE1A7F9B8EE7EB4A7C0F9E162BCE33576B315ECECBB6406837BF51F5 in
-  assert_norm (y < prime); y
-
-let base_point : jacob_point = (g_x, g_y, one)
-
-val is_point_on_curve: jacob_point -> bool
-let is_point_on_curve p =
-  let (x, y, z) = p in
-  y *% y = x *% x *% x +% a_coeff *% x +% b_coeff
-
-//------------------------------------
-// TODO: clean up
-let isPointAtInfinity (p:point_nat) =
-  let (_, _, z) = p in z = 0
-
-val toJacobianCoordinates: tuple2 nat nat -> tuple3 nat nat nat
-let toJacobianCoordinates (r0, r1) = (r0, r1, 1)
-//------------------------------------
-
-// TODO: avoid computing finv twice
-let norm_jacob_point (p:jacob_point) : jacob_point =
-  let (x, y, z) = p in
-  let z2 = z *% z in
-  let z3 = z2 *% z in
-  let z2i = finv z2 in
-  let z3i = finv z3 in
-  let x3 = z2i *% x in
-  let y3 = z3i *% y in
-  let z3 = if isPointAtInfinity (x, y, z) then zero else one in
-  (x3, y3, z3)
-
-
-///  Point addition and doubling in jacobian coordinates
-// TODO: use complete formulas
-
-let point_double (p:jacob_point) : jacob_point =
-  let x, y, z = p in
-  let delta = z *% z in
-  let gamma = y *% y in
-  let beta = x *% gamma in
-  let alpha = 3 *% (x -% delta) *% (x +% delta) in
-  let x3 = alpha *% alpha -% 8 *% beta in
-  let y3 = alpha *% (4 *% beta -% x3) -% 8 *% gamma *% gamma in
-  let z3 = (y +% z) *% (y +% z) -% delta -% gamma in
-  (x3, y3, z3)
-
-
-let point_add (p:jacob_point) (q:jacob_point) : jacob_point =
-  let (x1, y1, z1) = p in
-  let (x2, y2, z2) = q in
-
-  let z2z2 = z2 *% z2 in
-  let z1z1 = z1 *% z1 in
-
-  let u1 = x1 *% z2z2 in
-  let u2 = x2 *% z1z1 in
-
-  let s1 = y1 *% z2 *% z2z2 in
-  let s2 = y2 *% z1 *% z1z1 in
-
-  let h = u2 -% u1 in
-  let r = s2 -% s1 in
-
-  let rr = r *% r in
-  let hh = h *% h in
-  let hhh = h *% h *% h in
-
-  let x3 = rr -% hhh -% 2 *% u1 *% hh in
-  let y3 = r *% (u1 *% hh -% x3) -% s1 *% hhh in
-  let z3 = h *% z1 *% z2 in
-  if z2 = zero then (x1, y1, z1)
-  else
-    if z1 = zero then (x2, y2, z2)
-    else (x3, y3, z3)
-
+(** https://eprint.iacr.org/2013/816.pdf *)
 
 ///  Elliptic curve scalar multiplication
 // TODO: use Lib.Exponentiation
@@ -225,3 +68,197 @@ let secret_to_public k =
   let pai = (0, 0, 0) in
   let q, f = montgomery_ladder_spec k (pai, base_point) in
   norm_jacob_point q
+
+// from Spec.ECDSA.fst
+
+val validate_pubkey_point: publicKey:tuple3 nat nat nat{~(isPointAtInfinity publicKey)} -> bool
+let validate_pubkey_point publicKey =
+  let x, y, z = publicKey in
+  x < prime && y < prime && z < prime &&
+  is_point_on_curve (x, y, z)
+
+
+val checkCoordinates: r:nat -> s:nat -> bool
+let checkCoordinates r s =
+  if 0 < r && r < order && 0 < s && s < order then true else false
+
+
+type hash_alg_ecdsa =
+  | NoHash
+  | Hash of (a:hash_alg{a == SHA2_256 \/ a == SHA2_384 \/ a == SHA2_512})
+
+
+let invert_state_s (a:hash_alg_ecdsa): Lemma
+  (requires True)
+  (ensures (inversion hash_alg_ecdsa))
+  [ SMTPat (hash_alg_ecdsa) ]
+=
+  allow_inversion (hash_alg_ecdsa)
+
+
+val min_input_length: hash_alg_ecdsa -> Tot int
+let min_input_length a = match a with | NoHash -> 32 | Hash a -> 0
+
+(* let hash_length (a:hash_alg_ecdsa) = match a with | NoHash -> 32 | Hash a -> hash_length a *)
+
+
+val hashSpec:
+    a:hash_alg_ecdsa
+  -> mLen:size_nat{mLen >= min_input_length a}
+  -> m:lseq uint8 mLen ->
+  Tot (r:Lib.ByteSequence.lbytes
+    (if Hash? a then hash_length (match a with Hash a -> a) else mLen){length r >= 32})
+
+let hashSpec a mLen m =
+  assert_norm (pow2 32 < pow2 61);
+  assert_norm (pow2 32 < pow2 125);
+  allow_inversion hash_alg_ecdsa;
+  match a with
+  | NoHash -> m
+  | Hash a -> Spec.Agile.Hash.hash a m
+
+
+// TODO: rm, once we use complete point addition and doubling
+(**
+  Important changed was done comparing to the previous version:
+  The point addition routine used in the code doesnot work correctly in case the points are equal to each other. In this case the produced result is equal to 0. To solve it, before the execution we check that points are equal and then call either point double, if the points are identical, or point add.
+
+  Sage script:
+
+  prime = 2** 256 - 2**224 + 2**192 + 2**96 -1
+
+  def pointAdd(x1, y1, z1, x2, y2, z2):
+    z2z2 = z2 * z2
+    z1z1 = z1 * z1
+    u1 = x1 * z2 * z2
+    u2 = x2 * z1 * z1
+    s1 = y1 * z2 * z2 * z2
+    s2 = y2 * z1 * z1 * z1
+    h = u2 - u1
+    r = s2 - s1
+    rr = r * r
+    hh = h * h
+    hhh = h * h * h
+    x3 = (rr - hhh - 2 * u1 * hh) % prime
+    y3 = (r * (u1 * hh - x3) - s1 * hhh) % prime
+    z3 = (h * z1 * z2) % prime
+    return x3, y3, z3
+
+    pointAdd(94616602910890750895476491097843493117917747793373442062816991926475923005642,
+    36020885031736900871498807428940761284168967909318796815085487081314546588335, 1,
+    94616602910890750895476491097843493117917747793373442062816991926475923005642,
+    36020885031736900871498807428940761284168967909318796815085487081314546588335, 1)
+
+    The result is (0, 0, 0)
+
+    The correct result:
+
+    prime = 2** 256 - 2**224 + 2**192 + 2**96 -1
+    p = Zmod(prime)
+    a = -3
+    b = 41058363725152142129326129780047268409114441015993725554835256314039467401291
+
+    c = EllipticCurve(p, [a, b])
+
+    point = c(94616602910890750895476491097843493117917747793373442062816991926475923005642, 36020885031736900871498807428940761284168967909318796815085487081314546588335)
+    doublePoint = point + point
+
+    (50269061329272915414642095420870671498020143477290467295126614723791645001065, 13163180605447792593340701861458269296763094398473012191314473475747756843689)
+
+**)
+
+
+val ecdsa_verification_agile:
+    alg:hash_alg_ecdsa
+  -> publicKey:tuple2 nat nat
+  -> r:nat
+  -> s:nat
+  -> mLen:size_nat{mLen >= min_input_length alg}
+  -> m:lseq uint8 mLen
+  -> bool
+
+let ecdsa_verification_agile alg publicKey r s mLen m =
+  allow_inversion hash_alg_ecdsa;
+  let publicJacobian = toJacobianCoordinates publicKey in
+  if not (validate_pubkey_point publicJacobian) then false
+  else begin
+    if not (checkCoordinates r s) then false
+    else begin
+      let hashM = hashSpec alg mLen m in
+      let cutHashM = sub hashM 0 32 in
+      let hashNat = BSeq.nat_from_bytes_be cutHashM % order in
+
+      let sinv = qinv s in
+      let u1 = BSeq.nat_to_bytes_be 32 (sinv *^ hashNat) in
+      let u2 = BSeq.nat_to_bytes_be 32 (sinv *^ r) in
+
+      let pointAtInfinity = (0, 0, 0) in
+      let u1D, _ = montgomery_ladder_spec u1 (pointAtInfinity, base_point) in
+      let u2D, _ = montgomery_ladder_spec u2 (pointAtInfinity, publicJacobian) in
+      let sumD = if norm_jacob_point u1D = norm_jacob_point u2D then
+        point_double u1D
+      else
+        point_add u1D u2D in
+      let pointNorm = norm_jacob_point sumD in
+
+      let x, y, z = pointNorm in
+      let x = x % order in
+      if Spec.P256.isPointAtInfinity pointNorm then false else x = r
+    end
+  end
+
+
+val ecdsa_signature_agile:
+    alg:hash_alg_ecdsa
+  -> mLen:size_nat{mLen >= min_input_length alg}
+  -> m:lseq uint8 mLen
+  -> privateKey:lseq uint8 32
+  -> k:lseq uint8 32
+  -> tuple3 nat nat bool
+
+let ecdsa_signature_agile alg mLen m privateKey k =
+  assert_norm (pow2 32 < pow2 61);
+  assert_norm (pow2 32 < pow2 125);
+  let r, _ = montgomery_ladder_spec k ((0,0,0), base_point) in
+  let (xN, _, _) = norm_jacob_point r in
+
+  let hashM = hashSpec alg mLen m in
+  let cutHashM = sub hashM 0 32 in
+  let z = BSeq.nat_from_bytes_be cutHashM % order in
+
+  let kFelem = BSeq.nat_from_bytes_be k in
+  let privateKeyFelem = BSeq.nat_from_bytes_be privateKey in
+  let resultR = xN % order in
+  let resultS = (z + resultR * privateKeyFelem) * pow kFelem (order - 2) % order in
+  if resultR = 0 || resultS = 0 then
+    resultR, resultS, false
+  else
+    resultR, resultS, true
+
+// from Spec.DH
+
+(* Initiator *)
+val ecp256_dh_i: s:BSeq.lbytes 32 -> tuple3 (BSeq.lbytes 32) (BSeq.lbytes 32) bool
+let ecp256_dh_i s =
+  let xN, yN, zN = secret_to_public s in
+  if isPointAtInfinity (xN, yN, zN) then
+    BSeq.nat_to_bytes_be 32 xN, BSeq.nat_to_bytes_be 32 yN, false
+  else
+    BSeq.nat_to_bytes_be 32 xN, BSeq.nat_to_bytes_be 32 yN, true
+
+
+(* Responder *)
+val ecp256_dh_r: x:BSeq.lbytes 32 -> y:BSeq.lbytes 32 -> s:BSeq.lbytes 32
+  -> tuple3 (BSeq.lbytes 32) (BSeq.lbytes 32) bool
+
+let ecp256_dh_r x y s =
+  let x_, y_ = BSeq.nat_from_bytes_be x, BSeq.nat_from_bytes_be y in
+  let pointJacX, pointJacY, pointJacZ = toJacobianCoordinates (x_, y_) in
+  if validate_pubkey_point (pointJacX, pointJacY, pointJacZ) then
+    let xN, yN, zN = scalar_multiplication s (pointJacX, pointJacY, pointJacZ) in
+    if isPointAtInfinity (xN, yN, zN) then
+      BSeq.nat_to_bytes_be 32 xN, BSeq.nat_to_bytes_be 32 yN, false
+    else
+      BSeq.nat_to_bytes_be 32 xN, BSeq.nat_to_bytes_be 32 yN, true
+  else
+    BSeq.nat_to_bytes_be 32 0, BSeq.nat_to_bytes_be 32 0, false
