code/ecdsap256/Hacl.Impl.P256.PointAdd.fst
@@ -373,8 +373,8 @@ let point_add_if_second_branch_impl result p q u1 u2 s1 s2 r h uh hCube tempBuff
   lemma_point_add_1 (hD * hD * u1D) x3D rD s1D (hD * hD * hD);
   assert_by_tactic (s1D * (hD * hD * hD) == s1D * hD * hD * hD) canon;
 
-  assert_norm (S.modp_inv2 (pow2 256) > 0);
-  assert_norm (S.modp_inv2 (pow2 256) % S.prime <> 0);
+  assert_norm (S.modp_inv2_prime (pow2 256) S.prime > 0);
+  assert_norm (S.modp_inv2_prime (pow2 256) S.prime % S.prime <> 0);
 
   lemma_multiplication_not_mod_prime (as_nat h0 pZ);
   lemma_multiplication_not_mod_prime (as_nat h0 qZ);
