code/ecdsap256/Hacl.Impl.P256.Qinv.fsti
@@ -12,7 +12,6 @@ open Hacl.Spec.P256.Felem
 open Hacl.Impl.P256.Scalar
 
 module S = Spec.P256
-module SD = Spec.ECDSA
 
 #set-options "--z3rlimit 30 --fuel 0 --ifuel 0"
 
