code/ecdsap256/Hacl.Spec.P256.MontgomeryMultiplication.fst
@@ -7,7 +7,7 @@ module S = Spec.P256
 #set-options "--z3rlimit 40 --fuel 0 --ifuel 0"
 
 let mont_R = pow2 256
-let mont_R_inv = S.modp_inv2 (pow2 256)
+let mont_R_inv = S.modp_inv2_prime (pow2 256) S.prime
 
 let fromDomain_ (a:int) : S.felem = a * mont_R_inv % S.prime
 let toDomain_   (a:int) : S.felem = a * mont_R % S.prime
