specs/Spec.Agile.DH.fst
@@ -53,7 +53,7 @@ let dh a s p =
         let output = Spec.Curve25519.scalarmult s p in
         not (lbytes_eq (create (size_public a) (u8 0)) output), output
     | DH_P256 ->
-        let xN, yN, res = Spec.DH.ecp256_dh_r (sub p 0 32) (sub p 32 32) s in
+        let xN, yN, res = Spec.P256.ecp256_dh_r (sub p 0 32) (sub p 32 32) s in
         res, xN @| yN
   in
   if result then Some output else None
@@ -63,5 +63,5 @@ let secret_to_public a kpriv =
   match a with
   | DH_Curve25519 -> Some (Spec.Curve25519.secret_to_public kpriv)
   | DH_P256 ->
-      let xN, yN, res = Spec.DH.ecp256_dh_i kpriv in
+      let xN, yN, res = Spec.P256.ecp256_dh_i kpriv in
       if res then Some (xN @| yN) else None
