specs/ecdsap256/Spec.P256.PointOps.fst
@@ -1,0 +1,164 @@
+module Spec.P256.PointOps
+
+open FStar.Mul
+
+open Lib.IntTypes
+open Lib.Sequence
+
+module M = Lib.NatMod
+
+#set-options "--z3rlimit 50 --fuel 0 --ifuel 0"
+
+//---------------------------------------
+// TODO: remove
+val pow: a:nat -> b:nat -> nat
+let rec pow a b =
+  if b = 0 then 1 else a * (pow a (b - 1))
+
+type elem (n:pos) = x:nat{x < n}
+let mul_n (#n:pos) (x:elem n) (y:elem n) : elem n = (x * y) % n
+
+val exp: #n:pos -> a:elem n -> b:pos -> Tot (elem n) (decreases b)
+let rec exp #n a b =
+  if b = 1 then a
+  else
+    if b % 2 = 0 then exp (mul_n a a) (b / 2)
+    else mul_n a (exp (mul_n a a) (b / 2))
+
+let modp_inv2_prime (x:int) (p:nat{p > 3}) : elem p =
+  (exp #p (x % p) (p - 2)) % p
+//---------------------------------------
+
+///  Base field
+
+// 0xffffffff00000001000000000000000000000000ffffffffffffffffffffffff
+let prime: (a:pos{8 < a && a < pow2 256}) =
+  assert_norm (pow2 256 - pow2 224 + pow2 192 + pow2 96 - 1 > 8);
+  assert_norm (pow2 256 - pow2 224 + pow2 192 + pow2 96 - 1 < pow2 256);
+  pow2 256 - pow2 224 + pow2 192 + pow2 96 - 1
+
+let felem = x:nat{x < prime}
+let zero : felem = 0
+let one  : felem = 1
+
+let fadd (x y:felem) : felem = (x + y) % prime
+let fsub (x y:felem) : felem = (x - y) % prime
+let fmul (x y:felem) : felem = (x * y) % prime
+let finv (a:felem) : felem = M.pow_mod #prime a (prime - 2)
+let fsqrt (a:felem) : felem = M.pow_mod #prime a ((prime + 1) / 4)
+
+let ( +% ) = fadd
+let ( -% ) = fsub
+let ( *% ) = fmul
+
+
+///  Scalar field
+
+// Group order
+let order: (a:pos{a < pow2 256}) =
+  assert_norm (0xffffffff00000000ffffffffffffffffbce6faada7179e84f3b9cac2fc632551 < pow2 256);
+  0xffffffff00000000ffffffffffffffffbce6faada7179e84f3b9cac2fc632551
+
+let qelem = x:nat{x < order}
+let qadd (x y:qelem) : qelem = (x + y) % order
+let qmul (x y:qelem) : qelem = (x * y) % order
+let qinv (x:qelem) : qelem = M.pow_mod #order x (order - 2)
+
+let ( +^ ) = qadd
+let ( *^ ) = qmul
+
+
+///  Elliptic curve `y^2 = x^3 + a * x + b`
+
+let point_nat = tuple3 nat nat nat
+let jacob_point = p:point_nat{let (a, b, c) = p in
+  a < prime /\ b < prime /\ c < prime}
+
+// let aff_point = felem & felem           // Affine point
+// let jacob_point = felem & felem & felem // Jacobian coordinates
+
+let a_coeff : felem = (-3) % prime
+let b_coeff : felem =
+  assert_norm (41058363725152142129326129780047268409114441015993725554835256314039467401291 < prime);
+  41058363725152142129326129780047268409114441015993725554835256314039467401291
+
+// Base point
+let g_x : felem =
+  let x = 0x6B17D1F2E12C4247F8BCE6E563A440F277037D812DEB33A0F4A13945D898C296 in
+  assert_norm (x < prime); x
+let g_y : felem =
+  let y = 0x4FE342E2FE1A7F9B8EE7EB4A7C0F9E162BCE33576B315ECECBB6406837BF51F5 in
+  assert_norm (y < prime); y
+
+let base_point : jacob_point = (g_x, g_y, one)
+
+// TODO: fixme
+val is_point_on_curve: jacob_point -> bool
+let is_point_on_curve p =
+  let (x, y, z) = p in
+  y *% y = x *% x *% x +% a_coeff *% x +% b_coeff
+
+//------------------------------------
+// TODO: clean up
+let isPointAtInfinity (p:point_nat) =
+  let (_, _, z) = p in z = 0
+
+val toJacobianCoordinates: tuple2 nat nat -> tuple3 nat nat nat
+let toJacobianCoordinates (r0, r1) = (r0, r1, 1)
+//------------------------------------
+
+// TODO: avoid computing finv twice
+let norm_jacob_point (p:jacob_point) : jacob_point =
+  let (x, y, z) = p in
+  let z2 = z *% z in
+  let z3 = z2 *% z in
+  let z2i = finv z2 in
+  let z3i = finv z3 in
+  let x3 = z2i *% x in
+  let y3 = z3i *% y in
+  let z3 = if isPointAtInfinity (x, y, z) then zero else one in
+  (x3, y3, z3)
+
+
+///  Point addition and doubling in jacobian coordinates
+// TODO: use complete formulas
+
+let point_double (p:jacob_point) : jacob_point =
+  let x, y, z = p in
+  let delta = z *% z in
+  let gamma = y *% y in
+  let beta = x *% gamma in
+  let alpha = 3 *% (x -% delta) *% (x +% delta) in
+  let x3 = alpha *% alpha -% 8 *% beta in
+  let y3 = alpha *% (4 *% beta -% x3) -% 8 *% gamma *% gamma in
+  let z3 = (y +% z) *% (y +% z) -% delta -% gamma in
+  (x3, y3, z3)
+
+
+let point_add (p:jacob_point) (q:jacob_point) : jacob_point =
+  let (x1, y1, z1) = p in
+  let (x2, y2, z2) = q in
+
+  let z2z2 = z2 *% z2 in
+  let z1z1 = z1 *% z1 in
+
+  let u1 = x1 *% z2z2 in
+  let u2 = x2 *% z1z1 in
+
+  let s1 = y1 *% z2 *% z2z2 in
+  let s2 = y2 *% z1 *% z1z1 in
+
+  let h = u2 -% u1 in
+  let r = s2 -% s1 in
+
+  let rr = r *% r in
+  let hh = h *% h in
+  let hhh = h *% h *% h in
+
+  let x3 = rr -% hhh -% 2 *% u1 *% hh in
+  let y3 = r *% (u1 *% hh -% x3) -% s1 *% hhh in
+  let z3 = h *% z1 *% z2 in
+  if z2 = zero then (x1, y1, z1)
+  else
+    if z1 = zero then (x2, y2, z2)
+    else (x3, y3, z3)
